rename emp, star, valid_synth according to the paper

src/tls/Negotiation.Writers.Aux.fst
@@ -15,11 +15,11 @@ module LP = LowParse.Spec
 
 let valid_pskBinderEntry_intro =
    [@inline_let] let _ = assert_norm (Parsers.PskBinderEntry.pskBinderEntry == LowParse.Spec.Bytes.parse_bounded_vlbytes_t 32 255) in
-   LWP.valid_synth_parser_eq (LWP.parse_vlbytes 32ul 255ul) Parsers.PskBinderEntry.lwp_pskBinderEntry
+   LWP.valid_rewrite_parser_eq (LWP.parse_vlbytes 32ul 255ul) Parsers.PskBinderEntry.lwp_pskBinderEntry
 
 let valid_pskBinderEntry_elim =
    [@inline_let] let _ = assert_norm (Parsers.PskBinderEntry.pskBinderEntry == LowParse.Spec.Bytes.parse_bounded_vlbytes_t 32 255) in
-   LWP.valid_synth_parser_eq Parsers.PskBinderEntry.lwp_pskBinderEntry (LWP.parse_vlbytes 32ul 255ul)
+   LWP.valid_rewrite_parser_eq Parsers.PskBinderEntry.lwp_pskBinderEntry (LWP.parse_vlbytes 32ul 255ul)
 
 let valid_pskIdentity_intro =
   let open Parsers.PskIdentity in
@@ -27,98 +27,98 @@ let valid_pskIdentity_intro =
   assert_norm (pskIdentity_parser_kind == pskIdentity'_parser_kind);
   synth_pskIdentity_injective ();
   synth_pskIdentity_inverse ();
-  LWP.valid_synth_implies _ _ _ _
-  (LWP.valid_synth_compose
+  LWP.valid_rewrite_implies _ _ _ _
+  (LWP.valid_rewrite_compose
     _ _ _ _
-    (LWP.valid_synth_parse_synth (lwp_pskIdentity_identity `LWP.star` LWP.parse_u32) synth_pskIdentity synth_pskIdentity_recip ())
+    (LWP.valid_rewrite_parse_synth (lwp_pskIdentity_identity `LWP.parse_pair` LWP.parse_u32) synth_pskIdentity synth_pskIdentity_recip ())
     _ _ _
-    (LWP.valid_synth_parser_eq (LWP.parse_synth (lwp_pskIdentity_identity `LWP.star` LWP.parse_u32) synth_pskIdentity synth_pskIdentity_recip) lwp_pskIdentity)
+    (LWP.valid_rewrite_parser_eq (LWP.parse_synth (lwp_pskIdentity_identity `LWP.parse_pair` LWP.parse_u32) synth_pskIdentity synth_pskIdentity_recip) lwp_pskIdentity)
   )
   _ _
 
 
 let valid_offeredPsks_binders_intro =
   let open Parsers.OfferedPsks_binders in
-  LWP.valid_synth_implies _ _ _ _
-    (LWP.valid_synth_compose
+  LWP.valid_rewrite_implies _ _ _ _
+    (LWP.valid_rewrite_compose
       _ _ _ _
-      (LWP.valid_synth_parse_synth (LWP.parse_vllist Parsers.PskBinderEntry.lwp_pskBinderEntry 33ul 65535ul) synth_offeredPsks_binders synth_offeredPsks_binders_recip ())
+      (LWP.valid_rewrite_parse_synth (LWP.parse_vllist Parsers.PskBinderEntry.lwp_pskBinderEntry 33ul 65535ul) synth_offeredPsks_binders synth_offeredPsks_binders_recip ())
       _ _ _
-      (LWP.valid_synth_parser_eq _ _)
+      (LWP.valid_rewrite_parser_eq _ _)
     )
     _ _
 
 let valid_offeredPsks_binders_elim =
   let open Parsers.OfferedPsks_binders in
-  LWP.valid_synth_implies _ _ _ _
-    (LWP.valid_synth_compose
+  LWP.valid_rewrite_implies _ _ _ _
+    (LWP.valid_rewrite_compose
       _ _ _ _
-      (LWP.valid_synth_parser_eq _ _)
+      (LWP.valid_rewrite_parser_eq _ _)
       _ _ _
-      (LWP.valid_synth_parse_synth_recip (LWP.parse_vllist Parsers.PskBinderEntry.lwp_pskBinderEntry 33ul 65535ul) synth_offeredPsks_binders synth_offeredPsks_binders_recip ())
+      (LWP.valid_rewrite_parse_synth_recip (LWP.parse_vllist Parsers.PskBinderEntry.lwp_pskBinderEntry 33ul 65535ul) synth_offeredPsks_binders synth_offeredPsks_binders_recip ())
     )
     _ _
 
 let valid_offeredPsks_identities_intro =
   let open Parsers.OfferedPsks_identities in
-  LWP.valid_synth_implies _ _ _ _
-    (LWP.valid_synth_compose
+  LWP.valid_rewrite_implies _ _ _ _
+    (LWP.valid_rewrite_compose
       _ _ _ _
-      (LWP.valid_synth_parse_synth (LWP.parse_vllist Parsers.PskIdentity.lwp_pskIdentity 7ul 65535ul) synth_offeredPsks_identities synth_offeredPsks_identities_recip ())
+      (LWP.valid_rewrite_parse_synth (LWP.parse_vllist Parsers.PskIdentity.lwp_pskIdentity 7ul 65535ul) synth_offeredPsks_identities synth_offeredPsks_identities_recip ())
       _ _ _
-      (LWP.valid_synth_parser_eq _ _)
+      (LWP.valid_rewrite_parser_eq _ _)
     )
     _ _
 
 let valid_offeredPsks_identities_elim =
   let open Parsers.OfferedPsks_identities in
-  LWP.valid_synth_implies _ _ _ _
-    (LWP.valid_synth_compose
+  LWP.valid_rewrite_implies _ _ _ _
+    (LWP.valid_rewrite_compose
       _ _ _ _
-      (LWP.valid_synth_parser_eq _ _)
+      (LWP.valid_rewrite_parser_eq _ _)
       _ _ _
-      (LWP.valid_synth_parse_synth_recip (LWP.parse_vllist Parsers.PskIdentity.lwp_pskIdentity 7ul 65535ul) synth_offeredPsks_identities synth_offeredPsks_identities_recip ())
+      (LWP.valid_rewrite_parse_synth_recip (LWP.parse_vllist Parsers.PskIdentity.lwp_pskIdentity 7ul 65535ul) synth_offeredPsks_identities synth_offeredPsks_identities_recip ())
     )
     _ _
 
 let valid_offeredPsks_intro =
   let open Parsers.OfferedPsks in
-  LWP.valid_synth_implies _ _ _ _
-    (LWP.valid_synth_compose
+  LWP.valid_rewrite_implies _ _ _ _
+    (LWP.valid_rewrite_compose
       _ _ _ _
-      (LWP.valid_synth_parse_synth (lwp_offeredPsks_identities `LWP.star` lwp_offeredPsks_binders) synth_offeredPsks synth_offeredPsks_recip ())
+      (LWP.valid_rewrite_parse_synth (lwp_offeredPsks_identities `LWP.parse_pair` lwp_offeredPsks_binders) synth_offeredPsks synth_offeredPsks_recip ())
       _ _ _
-      (LWP.valid_synth_parser_eq _ _)
+      (LWP.valid_rewrite_parser_eq _ _)
     )
   _ _
 
 let valid_clientHelloExtension_CHE_pre_shared_key_intro =
   let open Parsers.ClientHelloExtension_CHE_pre_shared_key in
   Classical.forall_intro Parsers.PreSharedKeyClientExtension.preSharedKeyClientExtension_bytesize_eq;
-  LWP.valid_synth_implies _ _ _ _
-    (LWP.valid_synth_compose
+  LWP.valid_rewrite_implies _ _ _ _
+    (LWP.valid_rewrite_compose
       _ _ _ _
-      (LWP.valid_synth_parse_synth (LWP.parse_vldata Parsers.PreSharedKeyClientExtension.lwp_preSharedKeyClientExtension 0ul 65535ul) synth_clientHelloExtension_CHE_pre_shared_key synth_clientHelloExtension_CHE_pre_shared_key_recip ())
+      (LWP.valid_rewrite_parse_synth (LWP.parse_vldata Parsers.PreSharedKeyClientExtension.lwp_preSharedKeyClientExtension 0ul 65535ul) synth_clientHelloExtension_CHE_pre_shared_key synth_clientHelloExtension_CHE_pre_shared_key_recip ())
       _ _ _
-      (LWP.valid_synth_parser_eq _ _)
+      (LWP.valid_rewrite_parser_eq _ _)
     )
   _ _
 
-let valid_synth_pskKeyExchangeModes_intro =
+let valid_rewrite_pskKeyExchangeModes_intro =
 //  [@inline_let] let _ = assert_norm (LP.vldata_vlarray_precond 1 255 Parsers.PskKeyExchangeMode.pskKeyExchangeMode_parser 1 255 == true) in
-  LWP.valid_synth_parse_vlarray_intro
+  LWP.valid_rewrite_parse_vlarray_intro
     _
     Parsers.PskKeyExchangeMode.lwp_pskKeyExchangeMode
     1ul 255ul 1 255 ()
 
-let valid_synth_pskKeyExchangeModes_elim =
-  LWP.valid_synth_parse_vlarray_elim
+let valid_rewrite_pskKeyExchangeModes_elim =
+  LWP.valid_rewrite_parse_vlarray_elim
     _
     Parsers.PskKeyExchangeMode.lwp_pskKeyExchangeMode
     1ul 255ul 1 255 ()
 
 let valid_clientHelloExtension_CHE_psk_key_exchange_modes_intro =
-  LWP.valid_synth_parse_bounded_vldata_intro _ _ _ _
+  LWP.valid_rewrite_parse_bounded_vldata_intro _ _ _ _
 
 let valid_clientHelloExtension_CHE_early_data_intro =
-  LWP.valid_synth_parse_bounded_vldata_intro _ _ _ _
+  LWP.valid_rewrite_parse_bounded_vldata_intro _ _ _ _
