src/tls/Negotiation.Writers.Aux.fsti
@@ -5,11 +5,11 @@ module Negotiation.Writers.Aux
 module LWP = LowParseWriters.Parsers
 module LPI = LowParse.Low.Int
 
-val valid_pskBinderEntry_intro : LWP.valid_synth_t (LWP.parse_vlbytes 32ul 255ul) Parsers.PskBinderEntry.lwp_pskBinderEntry (fun _ -> True) (fun x -> x)
+val valid_pskBinderEntry_intro : LWP.valid_rewrite_t (LWP.parse_vlbytes 32ul 255ul) Parsers.PskBinderEntry.lwp_pskBinderEntry (fun _ -> True) (fun x -> x)
 
-val valid_pskBinderEntry_elim : LWP.valid_synth_t Parsers.PskBinderEntry.lwp_pskBinderEntry (LWP.parse_vlbytes 32ul 255ul) (fun _ -> True) (fun x -> x)
+val valid_pskBinderEntry_elim : LWP.valid_rewrite_t Parsers.PskBinderEntry.lwp_pskBinderEntry (LWP.parse_vlbytes 32ul 255ul) (fun _ -> True) (fun x -> x)
 
-val valid_pskIdentity_intro : LWP.valid_synth_t (Parsers.PskIdentity.lwp_pskIdentity_identity `LWP.star` LWP.parse_u32) Parsers.PskIdentity.lwp_pskIdentity (fun _ -> True) (fun (identity, age) -> { Parsers.PskIdentity.identity = identity; Parsers.PskIdentity.obfuscated_ticket_age = age; })
+val valid_pskIdentity_intro : LWP.valid_rewrite_t (Parsers.PskIdentity.lwp_pskIdentity_identity `LWP.parse_pair` LWP.parse_u32) Parsers.PskIdentity.lwp_pskIdentity (fun _ -> True) (fun (identity, age) -> { Parsers.PskIdentity.identity = identity; Parsers.PskIdentity.obfuscated_ticket_age = age; })
 
 let rec offeredPsks_binders_list_bytesize_correct
   (l: list Parsers.PskBinderEntry.pskBinderEntry)
@@ -22,13 +22,13 @@ let rec offeredPsks_binders_list_bytesize_correct
     Parsers.PskBinderEntry.pskBinderEntry_bytesize_eq a;
     offeredPsks_binders_list_bytesize_correct q
 
-val valid_offeredPsks_binders_intro : LWP.valid_synth_t
+val valid_offeredPsks_binders_intro : LWP.valid_rewrite_t
   (LWP.parse_vllist Parsers.PskBinderEntry.lwp_pskBinderEntry 33ul 65535ul)
   Parsers.OfferedPsks.lwp_offeredPsks_binders
   (fun _ -> True)
   (fun x -> x)
 
-val valid_offeredPsks_binders_elim : LWP.valid_synth_t
+val valid_offeredPsks_binders_elim : LWP.valid_rewrite_t
   Parsers.OfferedPsks.lwp_offeredPsks_binders
   (LWP.parse_vllist Parsers.PskBinderEntry.lwp_pskBinderEntry 33ul 65535ul)
   (fun _ -> True)
@@ -45,20 +45,20 @@ let rec offeredPsks_identities_list_bytesize_correct
     Parsers.PskIdentity.pskIdentity_bytesize_eq a;
     offeredPsks_identities_list_bytesize_correct q
 
-val valid_offeredPsks_identities_intro : LWP.valid_synth_t
+val valid_offeredPsks_identities_intro : LWP.valid_rewrite_t
   (LWP.parse_vllist Parsers.PskIdentity.lwp_pskIdentity 7ul 65535ul)
   Parsers.OfferedPsks.lwp_offeredPsks_identities
   (fun _ -> True)
   (fun x -> x)
 
-val valid_offeredPsks_identities_elim : LWP.valid_synth_t
+val valid_offeredPsks_identities_elim : LWP.valid_rewrite_t
   Parsers.OfferedPsks.lwp_offeredPsks_identities
   (LWP.parse_vllist Parsers.PskIdentity.lwp_pskIdentity 7ul 65535ul)
   (fun _ -> True)
   (fun x -> x)
 
-val valid_offeredPsks_intro : LWP.valid_synth_t
-  (Parsers.OfferedPsks.lwp_offeredPsks_identities `LWP.star` Parsers.OfferedPsks.lwp_offeredPsks_binders) 
+val valid_offeredPsks_intro : LWP.valid_rewrite_t
+  (Parsers.OfferedPsks.lwp_offeredPsks_identities `LWP.parse_pair` Parsers.OfferedPsks.lwp_offeredPsks_binders) 
   Parsers.OfferedPsks.lwp_offeredPsks
   (fun _ -> True)
   (fun (identities, binders) -> {
@@ -71,14 +71,14 @@ noextract
 let offeredPsks_intro
   (#inv: LWP.memory_invariant)
   #identities_pre #identities_post #identities_post_err
-  ($identities: (unit -> LWP.EWrite unit LWP.emp Parsers.OfferedPsks.lwp_offeredPsks_identities identities_pre identities_post identities_post_err inv))
+  ($identities: (unit -> LWP.EWrite unit LWP.parse_empty Parsers.OfferedPsks.lwp_offeredPsks_identities identities_pre identities_post identities_post_err inv))
   #binders_pre #binders_post #binders_post_err
-  ($binders: (unit -> LWP.EWrite unit LWP.emp Parsers.OfferedPsks.lwp_offeredPsks_binders binders_pre binders_post binders_post_err inv))
+  ($binders: (unit -> LWP.EWrite unit LWP.parse_empty Parsers.OfferedPsks.lwp_offeredPsks_binders binders_pre binders_post binders_post_err inv))
   ()
 :
   LWP.EWrite
     unit
-    LWP.emp
+    LWP.parse_empty
     Parsers.OfferedPsks.lwp_offeredPsks
     (fun _ -> identities_pre () /\ binders_pre ())
     (fun _ _ x ->
@@ -105,25 +105,25 @@ let offeredPsks_intro
 =
   LWP.recast_writer _ _ _ _ _ _ _ identities;
   LWP.frame _ _ _ _ _ _ _ (fun _ -> LWP.recast_writer _ _ _ _ _ _ _ binders);
-  LWP.valid_synth _ _ _ _ _ valid_offeredPsks_intro
+  LWP.valid_rewrite _ _ _ _ _ valid_offeredPsks_intro
 
-let valid_preSharedKeyClientExtension_intro : LWP.valid_synth_t
+let valid_preSharedKeyClientExtension_intro : LWP.valid_rewrite_t
   Parsers.OfferedPsks.lwp_offeredPsks
   Parsers.PreSharedKeyClientExtension.lwp_preSharedKeyClientExtension
   (fun _ -> True)
   (fun x -> x)
 =
   Parsers.PreSharedKeyClientExtension.preSharedKeyClientExtension_parser_serializer_eq ();
-  LWP.valid_synth_parser_eq _ _
+  LWP.valid_rewrite_parser_eq _ _
 
-let valid_preSharedKeyClientExtension_elim : LWP.valid_synth_t
+let valid_preSharedKeyClientExtension_elim : LWP.valid_rewrite_t
   Parsers.PreSharedKeyClientExtension.lwp_preSharedKeyClientExtension
   Parsers.OfferedPsks.lwp_offeredPsks
   (fun _ -> True)
   (fun x -> x)
 =
   Parsers.PreSharedKeyClientExtension.preSharedKeyClientExtension_parser_serializer_eq ();
-  LWP.valid_synth_parser_eq _ _
+  LWP.valid_rewrite_parser_eq _ _
 
 unfold
 let mk_clientHelloExtension_CHE_pre_shared_key_intro
@@ -132,7 +132,7 @@ let mk_clientHelloExtension_CHE_pre_shared_key_intro
 = Parsers.PreSharedKeyClientExtension.preSharedKeyClientExtension_bytesize_eq x;
   x
 
-val valid_clientHelloExtension_CHE_pre_shared_key_intro : LWP.valid_synth_t
+val valid_clientHelloExtension_CHE_pre_shared_key_intro : LWP.valid_rewrite_t
   (LWP.parse_vldata Parsers.PreSharedKeyClientExtension.lwp_preSharedKeyClientExtension 0ul 65535ul)
   Parsers.ClientHelloExtension.lwp_clientHelloExtension_CHE_pre_shared_key
   (fun _ -> True)
@@ -150,7 +150,7 @@ let clientHelloExtension_CHE_pre_shared_key_intro #inv () : LWP.Write
 =
   let x = LWP.get_state () in
   Parsers.PreSharedKeyClientExtension.preSharedKeyClientExtension_bytesize_eq x;
-  LWP.valid_synth _ _ _ _ _
+  LWP.valid_rewrite _ _ _ _ _
     valid_clientHelloExtension_CHE_pre_shared_key_intro
 
   (* NOTE: I could also define the elim but QuackyDucky already defines an accessor *)
@@ -166,19 +166,19 @@ let rec list_size_pskKeyExchangeMode
   | [] -> ()
   | a :: q -> list_size_pskKeyExchangeMode q
 
-val valid_synth_pskKeyExchangeModes_intro : LWP.valid_synth_t
+val valid_rewrite_pskKeyExchangeModes_intro : LWP.valid_rewrite_t
   (LWP.parse_vllist Parsers.PskKeyExchangeMode.lwp_pskKeyExchangeMode 1ul 255ul)
   Parsers.PskKeyExchangeModes.lwp_pskKeyExchangeModes
   (fun _ -> True)
   (fun x -> x)
 
-val valid_synth_pskKeyExchangeModes_elim : LWP.valid_synth_t
+val valid_rewrite_pskKeyExchangeModes_elim : LWP.valid_rewrite_t
   Parsers.PskKeyExchangeModes.lwp_pskKeyExchangeModes
   (LWP.parse_vllist Parsers.PskKeyExchangeMode.lwp_pskKeyExchangeMode 1ul 255ul)
   (fun _ -> True)
   (fun x -> x)
 
-val valid_clientHelloExtension_CHE_psk_key_exchange_modes_intro : LWP.valid_synth_t
+val valid_clientHelloExtension_CHE_psk_key_exchange_modes_intro : LWP.valid_rewrite_t
   (LWP.parse_vldata Parsers.PskKeyExchangeModes.lwp_pskKeyExchangeModes 0ul 65535ul)
   Parsers.ClientHelloExtension.lwp_clientHelloExtension_CHE_psk_key_exchange_modes
   (fun _ -> True)
@@ -186,8 +186,8 @@ val valid_clientHelloExtension_CHE_psk_key_exchange_modes_intro : LWP.valid_synt
     Parsers.PskKeyExchangeModes.pskKeyExchangeModes_bytesize_eq x;
     x)
 
-val valid_clientHelloExtension_CHE_early_data_intro : LWP.valid_synth_t
-  (LWP.parse_vldata LWP.emp 0ul 65535ul)
+val valid_clientHelloExtension_CHE_early_data_intro : LWP.valid_rewrite_t
+  (LWP.parse_vldata LWP.parse_empty 0ul 65535ul)
   Parsers.ClientHelloExtension.lwp_clientHelloExtension_CHE_early_data
   (fun _ -> True)
   (fun x -> x)
