src/tls/Negotiation.Writers.Aux2.fst
@@ -37,7 +37,7 @@ let che_enum : LWP.pparser _ _ _ (LP.serialize_maybe_enum_key _ che_dsum.LWP.dsu
 
 #restart-solver
 
-let valid_synth_constr_clientHelloExtension
+let valid_rewrite_constr_clientHelloExtension
   (k: Parsers.ExtensionType.extensionType { LP.list_mem k (LP.list_map fst Parsers.ExtensionType.extensionType_enum) })
   (p: LWP.pparser
        (Parsers.ClientHelloExtension.clientHelloExtension_case_of_extensionType k)
@@ -45,8 +45,8 @@ let valid_synth_constr_clientHelloExtension
        (dsnd (Parsers.ClientHelloExtension.parse_clientHelloExtension_cases k))
        (Parsers.ClientHelloExtension.serialize_clientHelloExtension_cases k)
   )
-: Tot (LWP.valid_synth_t
-  (Parsers.ExtensionType.lwp_extensionType `LWP.star` p)
+: Tot (LWP.valid_rewrite_t
+  (Parsers.ExtensionType.lwp_extensionType `LWP.parse_pair` p)
   Parsers.ClientHelloExtension.lwp_clientHelloExtension
   (fun (k', _) -> k' == k)
   (fun (_, ext) -> Parsers.ClientHelloExtension.synth_known_clientHelloExtension_cases k ext)
@@ -57,20 +57,20 @@ let valid_synth_constr_clientHelloExtension
   assert_norm (LP.parse_dsum_kind (LP.get_parser_kind extensionType_repr_parser) clientHelloExtension_sum parse_clientHelloExtension_cases (LP.get_parser_kind clientHelloExtension_CHE_default_parser) == clientHelloExtension_parser_kind);
   lemma_synth_extensionType_inj ();
   lemma_synth_extensionType_inv ();
-  LWP.valid_synth_implies _ _ _ _
-  (LWP.valid_synth_compose
+  LWP.valid_rewrite_implies _ _ _ _
+  (LWP.valid_rewrite_compose
     _ _ _ _
-    (LWP.valid_synth_star_compat_r
+    (LWP.valid_rewrite_parse_pair_compat_r
       _ _ _ _ _
-      (LWP.valid_synth_compose
+      (LWP.valid_rewrite_compose
         _ _ _ _
-        (LWP.valid_synth_parser_eq _ _)
+        (LWP.valid_rewrite_parser_eq _ _)
         _ _ _
-        (LWP.valid_synth_parse_synth_recip che_enum synth_extensionType synth_extensionType_inv ())
+        (LWP.valid_rewrite_parse_synth_recip che_enum synth_extensionType synth_extensionType_inv ())
       )
     )
     _ _ _
-    (LWP.valid_synth_parse_dsum_known
+    (LWP.valid_rewrite_parse_dsum_known
       che_dsum
       _
       _
@@ -84,26 +84,26 @@ let valid_synth_constr_clientHelloExtension
 
 #restart-solver
 
-let valid_synth_constr_clientHelloExtension_CHE_pre_shared_key =
+let valid_rewrite_constr_clientHelloExtension_CHE_pre_shared_key =
   let open Parsers.ClientHelloExtension in
   let open Parsers.ExtensionType in
   assert_norm (LP.list_mem Pre_shared_key (LP.list_map fst extensionType_enum) == true);
-  LWP.valid_synth_implies _ _ _ _
-    (valid_synth_constr_clientHelloExtension Pre_shared_key lwp_clientHelloExtension_CHE_pre_shared_key)
+  LWP.valid_rewrite_implies _ _ _ _
+    (valid_rewrite_constr_clientHelloExtension Pre_shared_key lwp_clientHelloExtension_CHE_pre_shared_key)
     _ _
 
-let valid_synth_constr_clientHelloExtension_CHE_psk_key_exchange_modes =
+let valid_rewrite_constr_clientHelloExtension_CHE_psk_key_exchange_modes =
   let open Parsers.ClientHelloExtension in
   let open Parsers.ExtensionType in
   assert_norm (LP.list_mem Psk_key_exchange_modes (LP.list_map fst extensionType_enum) == true);
-  LWP.valid_synth_implies _ _ _ _
-    (valid_synth_constr_clientHelloExtension Psk_key_exchange_modes lwp_clientHelloExtension_CHE_psk_key_exchange_modes)
+  LWP.valid_rewrite_implies _ _ _ _
+    (valid_rewrite_constr_clientHelloExtension Psk_key_exchange_modes lwp_clientHelloExtension_CHE_psk_key_exchange_modes)
     _ _
 
-let valid_synth_constr_clientHelloExtension_CHE_early_data =
+let valid_rewrite_constr_clientHelloExtension_CHE_early_data =
   let open Parsers.ClientHelloExtension in
   let open Parsers.ExtensionType in
   assert_norm (LP.list_mem Early_data (LP.list_map fst extensionType_enum) == true);
-  LWP.valid_synth_implies _ _ _ _
-    (valid_synth_constr_clientHelloExtension Early_data lwp_clientHelloExtension_CHE_early_data)
+  LWP.valid_rewrite_implies _ _ _ _
+    (valid_rewrite_constr_clientHelloExtension Early_data lwp_clientHelloExtension_CHE_early_data)
     _ _
