src/tls/Negotiation.Writers.Aux2.fsti
@@ -5,8 +5,8 @@ module Negotiation.Writers.Aux2
 module LWP = LowParseWriters.Parsers
 module LPI = LowParse.Low.Int
 
-val valid_synth_constr_clientHelloExtension_CHE_pre_shared_key : LWP.valid_synth_t
-  (Parsers.ExtensionType.lwp_extensionType `LWP.star` Parsers.ClientHelloExtension.lwp_clientHelloExtension_CHE_pre_shared_key)
+val valid_rewrite_constr_clientHelloExtension_CHE_pre_shared_key : LWP.valid_rewrite_t
+  (Parsers.ExtensionType.lwp_extensionType `LWP.parse_pair` Parsers.ClientHelloExtension.lwp_clientHelloExtension_CHE_pre_shared_key)
   Parsers.ClientHelloExtension.lwp_clientHelloExtension
   (fun (k, _) -> k == Parsers.ExtensionType.Pre_shared_key)
   (fun (_, ext) -> Parsers.ClientHelloExtension.CHE_pre_shared_key ext)
@@ -15,11 +15,11 @@ inline_for_extraction
 noextract
 let constr_clientHelloExtension_CHE_pre_shared_key
   #inv #pre #post #post_err
-  ($f: (unit -> LWP.EWrite unit LWP.emp Parsers.ClientHelloExtension.lwp_clientHelloExtension_CHE_pre_shared_key pre post post_err inv))
+  ($f: (unit -> LWP.EWrite unit LWP.parse_empty Parsers.ClientHelloExtension.lwp_clientHelloExtension_CHE_pre_shared_key pre post post_err inv))
   ()
 : LWP.EWrite
     unit
-    LWP.emp
+    LWP.parse_empty
     Parsers.ClientHelloExtension.lwp_clientHelloExtension
     (fun _ -> pre ())
     (fun _ _ msg ->
@@ -42,16 +42,16 @@ let constr_clientHelloExtension_CHE_pre_shared_key
     inv
 = LWP.start Parsers.ExtensionType.lwp_extensionType Parsers.ExtensionType.extensionType_writer Parsers.ExtensionType.Pre_shared_key;
   LWP.frame _ _ _ _ _ _ _ (fun _ -> LWP.recast_writer _ _ _ _ _ _ _ f);
-  LWP.valid_synth _ _ _ _ _ valid_synth_constr_clientHelloExtension_CHE_pre_shared_key
+  LWP.valid_rewrite _ _ _ _ _ valid_rewrite_constr_clientHelloExtension_CHE_pre_shared_key
 
 inline_for_extraction
 noextract
 let constr_clientHelloExtension_CHE_pre_shared_key'
   #inv
-  (f: (unit -> LWP.EWrite unit LWP.emp Parsers.ClientHelloExtension.lwp_clientHelloExtension_CHE_pre_shared_key (fun _ -> True) (fun _ _ _ -> True) (fun _ -> True) inv))
+  (f: (unit -> LWP.EWrite unit LWP.parse_empty Parsers.ClientHelloExtension.lwp_clientHelloExtension_CHE_pre_shared_key (fun _ -> True) (fun _ _ _ -> True) (fun _ -> True) inv))
 : LWP.EWrite
     unit
-    LWP.emp
+    LWP.parse_empty
     Parsers.ClientHelloExtension.lwp_clientHelloExtension
     (fun _ -> True)
     (fun _ _ msg ->
@@ -67,10 +67,10 @@ let constr_clientHelloExtension_CHE_pre_shared_key'
     inv
 = LWP.start Parsers.ExtensionType.lwp_extensionType Parsers.ExtensionType.extensionType_writer Parsers.ExtensionType.Pre_shared_key;
   LWP.frame _ _ _ _ _ _ _ (fun _ -> LWP.recast_writer _ _ _ _ _ _ _ f);
-  LWP.valid_synth _ _ _ _ _ valid_synth_constr_clientHelloExtension_CHE_pre_shared_key
+  LWP.valid_rewrite _ _ _ _ _ valid_rewrite_constr_clientHelloExtension_CHE_pre_shared_key
 
-val valid_synth_constr_clientHelloExtension_CHE_psk_key_exchange_modes : LWP.valid_synth_t
-  (Parsers.ExtensionType.lwp_extensionType `LWP.star` Parsers.ClientHelloExtension.lwp_clientHelloExtension_CHE_psk_key_exchange_modes)
+val valid_rewrite_constr_clientHelloExtension_CHE_psk_key_exchange_modes : LWP.valid_rewrite_t
+  (Parsers.ExtensionType.lwp_extensionType `LWP.parse_pair` Parsers.ClientHelloExtension.lwp_clientHelloExtension_CHE_psk_key_exchange_modes)
   Parsers.ClientHelloExtension.lwp_clientHelloExtension
   (fun (k, _) -> k == Parsers.ExtensionType.Psk_key_exchange_modes)
   (fun (_, ext) -> Parsers.ClientHelloExtension.CHE_psk_key_exchange_modes ext)
@@ -79,11 +79,11 @@ inline_for_extraction
 noextract
 let constr_clientHelloExtension_CHE_psk_key_exchange_modes
   #inv #pre #post #post_err
-  ($f: (unit -> LWP.EWrite unit LWP.emp Parsers.ClientHelloExtension.lwp_clientHelloExtension_CHE_psk_key_exchange_modes pre post post_err inv))
+  ($f: (unit -> LWP.EWrite unit LWP.parse_empty Parsers.ClientHelloExtension.lwp_clientHelloExtension_CHE_psk_key_exchange_modes pre post post_err inv))
   ()
 : LWP.EWrite
     unit
-    LWP.emp
+    LWP.parse_empty
     Parsers.ClientHelloExtension.lwp_clientHelloExtension
     (fun _ -> pre ())
     (fun _ _ msg ->
@@ -106,16 +106,16 @@ let constr_clientHelloExtension_CHE_psk_key_exchange_modes
     inv
 = LWP.start Parsers.ExtensionType.lwp_extensionType Parsers.ExtensionType.extensionType_writer Parsers.ExtensionType.Psk_key_exchange_modes;
   LWP.frame _ _ _ _ _ _ _ (fun _ -> LWP.recast_writer _ _ _ _ _ _ _ f);
-  LWP.valid_synth _ _ _ _ _ valid_synth_constr_clientHelloExtension_CHE_psk_key_exchange_modes
+  LWP.valid_rewrite _ _ _ _ _ valid_rewrite_constr_clientHelloExtension_CHE_psk_key_exchange_modes
 
 inline_for_extraction
 noextract
 let constr_clientHelloExtension_CHE_psk_key_exchange_modes'
   #inv
-  (f: (unit -> LWP.EWrite unit LWP.emp Parsers.ClientHelloExtension.lwp_clientHelloExtension_CHE_psk_key_exchange_modes (fun _ -> True) (fun _ _ _ -> True) (fun _ -> True) inv))
+  (f: (unit -> LWP.EWrite unit LWP.parse_empty Parsers.ClientHelloExtension.lwp_clientHelloExtension_CHE_psk_key_exchange_modes (fun _ -> True) (fun _ _ _ -> True) (fun _ -> True) inv))
 : LWP.EWrite
     unit
-    LWP.emp
+    LWP.parse_empty
     Parsers.ClientHelloExtension.lwp_clientHelloExtension
     (fun _ -> True)
     (fun _ _ msg ->
@@ -131,10 +131,10 @@ let constr_clientHelloExtension_CHE_psk_key_exchange_modes'
     inv
 = LWP.start Parsers.ExtensionType.lwp_extensionType Parsers.ExtensionType.extensionType_writer Parsers.ExtensionType.Psk_key_exchange_modes;
   LWP.frame _ _ _ _ _ _ _ (fun _ -> LWP.recast_writer _ _ _ _ _ _ _ f);
-  LWP.valid_synth _ _ _ _ _ valid_synth_constr_clientHelloExtension_CHE_psk_key_exchange_modes
+  LWP.valid_rewrite _ _ _ _ _ valid_rewrite_constr_clientHelloExtension_CHE_psk_key_exchange_modes
 
-val valid_synth_constr_clientHelloExtension_CHE_early_data : LWP.valid_synth_t
-  (Parsers.ExtensionType.lwp_extensionType `LWP.star` Parsers.ClientHelloExtension.lwp_clientHelloExtension_CHE_early_data)
+val valid_rewrite_constr_clientHelloExtension_CHE_early_data : LWP.valid_rewrite_t
+  (Parsers.ExtensionType.lwp_extensionType `LWP.parse_pair` Parsers.ClientHelloExtension.lwp_clientHelloExtension_CHE_early_data)
   Parsers.ClientHelloExtension.lwp_clientHelloExtension
   (fun (k, _) -> k == Parsers.ExtensionType.Early_data)
   (fun (_, ext) -> Parsers.ClientHelloExtension.CHE_early_data ext)
@@ -143,11 +143,11 @@ inline_for_extraction
 noextract
 let constr_clientHelloExtension_CHE_early_data
   #inv #pre #post #post_err
-  ($f: (unit -> LWP.EWrite unit LWP.emp Parsers.ClientHelloExtension.lwp_clientHelloExtension_CHE_early_data pre post post_err inv))
+  ($f: (unit -> LWP.EWrite unit LWP.parse_empty Parsers.ClientHelloExtension.lwp_clientHelloExtension_CHE_early_data pre post post_err inv))
   ()
 : LWP.EWrite
     unit
-    LWP.emp
+    LWP.parse_empty
     Parsers.ClientHelloExtension.lwp_clientHelloExtension
     (fun _ -> pre ())
     (fun _ _ msg ->
@@ -170,16 +170,16 @@ let constr_clientHelloExtension_CHE_early_data
     inv
 = LWP.start Parsers.ExtensionType.lwp_extensionType Parsers.ExtensionType.extensionType_writer Parsers.ExtensionType.Early_data;
   LWP.frame _ _ _ _ _ _ _ (fun _ -> LWP.recast_writer _ _ _ _ _ _ _ f);
-  LWP.valid_synth _ _ _ _ _ valid_synth_constr_clientHelloExtension_CHE_early_data
+  LWP.valid_rewrite _ _ _ _ _ valid_rewrite_constr_clientHelloExtension_CHE_early_data
 
 inline_for_extraction
 noextract
 let constr_clientHelloExtension_CHE_early_data'
   #inv
-  (f: (unit -> LWP.EWrite unit LWP.emp Parsers.ClientHelloExtension.lwp_clientHelloExtension_CHE_early_data (fun _ -> True) (fun _ _ _ -> True) (fun _ -> True) inv))
+  (f: (unit -> LWP.EWrite unit LWP.parse_empty Parsers.ClientHelloExtension.lwp_clientHelloExtension_CHE_early_data (fun _ -> True) (fun _ _ _ -> True) (fun _ -> True) inv))
 : LWP.EWrite
     unit
-    LWP.emp
+    LWP.parse_empty
     Parsers.ClientHelloExtension.lwp_clientHelloExtension
     (fun _ -> True)
     (fun _ _ msg ->
@@ -195,4 +195,4 @@ let constr_clientHelloExtension_CHE_early_data'
     inv
 = LWP.start Parsers.ExtensionType.lwp_extensionType Parsers.ExtensionType.extensionType_writer Parsers.ExtensionType.Early_data;
   LWP.frame _ _ _ _ _ _ _ (fun _ -> LWP.recast_writer _ _ _ _ _ _ _ f);
-  LWP.valid_synth _ _ _ _ _ valid_synth_constr_clientHelloExtension_CHE_early_data
+  LWP.valid_rewrite _ _ _ _ _ valid_rewrite_constr_clientHelloExtension_CHE_early_data
